Jrlean/HasTypeId/Derive.lean
@@ -30,7 +30,7 @@ def _root_.Lean.Expr.toSyntax := Term.exprToSyntax
 
 def generateNames (n : Nat) (suggestion : Name) : CoreM (Array Name) :=
   Array.range n
-  |>.mapM fun _ => mkFreshUserName suggestion
+  |>.mapM fun i => mkFreshUserName (suggestion.appendAfter <| toString i)
 
 /- A derive handler takes an array of names and elaborates commands that
    introduce the instance for them. We also need to add axioms that assume the
@@ -48,7 +48,7 @@ def derivingHandler : DerivingHandler := fun names => do
     match constant_info with
     | .inductInfo inductiveVal => do
       let (params, ret) ← readParameters inductiveVal
-      command name params
+      command name inductiveVal.levelParams params
     | .axiomInfo ..
     | .defnInfo ..
     | .thmInfo ..
@@ -59,36 +59,92 @@ def derivingHandler : DerivingHandler := fun names => do
       throwError m!"cannot derive TypeId for constant '{name}' as it is not definition of a new unique type. ConstantInfo object: {constant_info}"
   return true
 where
-  command (name : Name) (paramTypes : Array Expr) : CommandElabM Unit := do
+  command (name : Name) levelParams (paramTypes : Array Expr) : CommandElabM Unit := do
+    -- Filter the level parameters to only those that the parameter types depend
+    -- on. This is because having universe levels that only affect the return
+    -- type or nothing at all means a synthesis failure when we try to call the
+    -- typeId function.
+    -- let levelParams :=
+    --   levelParams.filter fun l => paramTypes.any fun t =>
+    --     dependsOn t l
     /-
     Does three things:
     1. declares a function called _.typeId
     2. declares an axiom _.typeId_ofType
     3. declares an instance of HasTypeId
     -/
+    -- First generate some names for the arguments.
     let paramNames ← liftCoreM <| generateNames paramTypes.size `a
-    let paramTypeIdTerms ← paramNames.mapM (fun name =>
-      `(HasTypeId.typeId $(mkIdent name))
-    )
     -- An expression that returns the type `TypeId`
     let typeIdType : Expr := .const ``TypeId []
+    -- An expression that returns the type `HasTypeId α`
+    let hasTypeIdType α := mkAppM ``HasTypeId #[α]
     -- Declare the type id
     liftCoreM <| addDecl (forceExpose := true) <| .defnDecl {
       name := name ++ `typeId
-      levelParams := [] -- TODO
-      type := ← liftCoreM <| mkArrowN paramTypes typeIdType -- TODO
-      value := ← liftTermElabM do
-        mkAppM ``TypeId.mk #[
+      levelParams := levelParams
+      type := ← liftTermElabM do
+        -- Declare the parameters
+        withLocalDeclsDND (paramNames.zip paramTypes) fun params => do
+        -- Declare the instances
+        withLocalDecls
+          (params.map (fun p => (.anonymous, .instImplicit, fun _ => hasTypeIdType p)))
+          fun paramInsts => do
+        mkForallFVars
+          (params.zip paramInsts |>.flatMap fun (a, b) => #[a, b])
+          typeIdType
+      value := ← liftTermElabM do -- TODO: This should take aruguments and match the type
+        -- Declare the parameters
+        withLocalDeclsDND (paramNames.zip paramTypes) fun params => do
+        -- Declare the instances
+        withLocalDecls
+          (params.map (fun p => (.anonymous, .instImplicit, fun _ => hasTypeIdType p)))
+          fun paramInsts => do
+        mkLambdaFVars
+          (params.zip paramInsts |>.flatMap fun (a, b) => #[a, b])
+          <| ← mkAppM ``TypeId.mk #[
           -- First argument is the constant's name
           toExpr name,
           -- The rest of the arguments are the names of the arguments to the
           -- constant.
-          ← mkListLit typeIdType <| ← paramTypes.toList.mapM fun t =>
-              mkAppM ``typeId #[t],
+          ← mkListLit typeIdType <| ← (params.zip paramInsts).toList.mapM fun (p, i) =>
+              mkAppOptM ``typeId #[some p, some i],
         ]
       hints := .regular 10
       safety := .safe
     }
+    -- Declare the axiom which states that the type id is correct.
+    liftCoreM <| addDecl <| .axiomDecl {
+      name := name ++ `typeId_ofType
+      levelParams := levelParams
+      type := ← liftTermElabM do
+        -- Declare the parameters
+        withLocalDeclsDND (paramNames.zip paramTypes) fun params => do
+        -- Declare the instances
+        withLocalDecls
+          (params.map (fun p => (.anonymous, .instImplicit, fun _ => hasTypeIdType p)))
+          fun paramInsts => do
+        let paramInterleavedInsts :=
+          (params.zip paramInsts |>.flatMap fun (a, b) => #[a, b])
+        mkForallFVars paramInterleavedInsts <|
+        ← mkAppM ``TypeId.OfType #[
+          -- First argument is the type id
+          ← mkAppM (name ++ `typeId) paramInterleavedInsts,
+          -- Second is the type
+          ← mkAppM name params,
+        ]
+      isUnsafe := false
+    }
+    -- Declare the instance of HasTypeId
+    liftCoreM <| addDecl <| .defnDecl {
+      name := name ++ `hasTypeId
+      levelParams := levelParams
+      type := ← liftTermElabM do sorry
+      value := ← liftTermElabM do sorry
+      hints := .regular 10
+      safety := .safe
+    }
+    liftCoreM <| Attribute.add (name ++ `hasTypeId) `instance (← getRef)
     -- `(
     --   def $typeIdIdent $paramBinders* : TypeId where
     --     name := $nameTerm
@@ -111,4 +167,4 @@ where
     if not t.isSort then throwError m!"type {x.name} is not a sort"
     return (params, t)
 
-initialize registerDerivingHandler ``TypeId derivingHandler
+initialize registerDerivingHandler ``HasTypeId derivingHandler
