Jrlean/HasTypeId/Instances.lean
@@ -6,5 +6,10 @@ meta import Jrlean.HasTypeId.Derive
 
 namespace Jrlean
 
-deriving instance TypeId for Nat, Int, String, Bool, PUnit
-deriving instance TypeId for List
+deriving instance HasTypeId for Nat, Int, String, Bool, PUnit
+#print PUnit.typeId
+#print PUnit.typeId_ofType
+deriving instance HasTypeId for List
+#print List.typeId
+#eval List.typeId Nat
+#eval List.typeId_ofType Nat
